**Theorem.** Let $A$, $B$, and $C$ be sets. Let $f:A\hookrightarrow B$ and $g:B\hookrightarrow C$. Then, $g\circ f:A\hookrightarrow C$.

**Proof.** Suppose $a,b\in A$, and suppose $g\circ f(a)=g\circ f(b)$. Then, by [[Evaluations of Composite Functions]] $g(f(a))=g(f(b))$. Since $g$ is injective, we have $f(a)=f(b)$. Since $f$ is injective, we have $a=b$. $\blacksquare$
***
Definitions used:
- [[Set]]
- [[Function]]
- [[Composition of Functions]]
- [[Injective Function]]

Theorems used:
- [[Evaluations of Composite Functions]]