**Theorem.** Let $\mathsf{C}$ be a category. Then, $$(\mathsf{C}^\text{op})^\text{op}=\mathsf{C}.$$
**Proof.** Objects in $(\mathsf{C}^\text{op})^\text{op}$ are the same as objects in $\mathsf{C}^\text{op}$, which are the same as objects in $\mathsf{C}$. A morphism $f:A\to B$ in $\mathsf{C}$ corresponds to a unique morphism $f^\text{op}:B\to A$ in $\mathsf{C}^\text{op}$, which corresponds to a unique morphism $(f^\text{op})^\text{op}:A\to B$ in $(\mathsf{C}^\text{op})^\text{op}$. Therefore, $\mathsf{C}$ and $(\mathsf{C}^\text{op})^\text{op}$ have identical objects and morphisms, so $\mathsf{C}=(\mathsf{C}^\text{op})^\text{op}$. $\blacksquare$
***
Definitions used:
- [[Category]]
- [[Opposite Category]]