**Theorem.** Let $R$ be a ring. Then, for all $a\in R$, $a\cdot 0=0$ and $0\cdot a=0$.

**Proof.** Suppose $a\in R$. We have
$$\begin{align}
a\cdot 0 +0& = a\cdot 0\\
 & =a\cdot(0+0) \\
 & =a\cdot 0+a\cdot 0,
\end{align}$$
so by [[Cancellation Properties on Groups]] $a\cdot 0=0$. Likewise,
$$\begin{align}
0\cdot a+0 & =0\cdot a \\
 & =(0+0)\cdot a \\
 & =0\cdot a+0\cdot a,
\end{align}$$
so by [[Cancellation Properties on Groups]] $0\cdot a=0$. $\blacksquare$
***
Definitions used:
- [[Ring]]

Theorems used:
- [[Cancellation Properties on Groups]]